src/program_logic/wp_nval.v
@@ -3,52 +3,6 @@ From Perennial.program_logic Require Export crash_weakestpre staged_invariant_al
 Set Default Proof Using "Type".
 Import uPred.
 
-Definition logical_step_emp `{!irisGS Λ Σ, !crashGS Σ} E D P : iProp Σ :=
-  ∀ Q, (|={E|D}⧗=> Q) -∗ (|={E|D}⧗=> Q ∗ P).
-Notation "|~{ E | D }~> P" := (logical_step_emp E D P) (at level 99, P at level 200, format "'[  ' |~{ E | D }~>  '/' P ']'").
-
-Lemma logical_step_emp_wand `{!irisGS Λ Σ, !crashGS Σ} E D P Q :
-  (|~{E|D}~> P) -∗  
-  (P -∗ Q) -∗
-  |~{E|D}~> Q.
-Proof.
-  iIntros "Hstep HPQ" (R) "HR".
-  iDestruct ("Hstep" with "HR") as "HR".
-  iApply (physical_step_wand with "HR"). iIntros "[$ P]".
-  by iApply "HPQ".
-Qed.
-
-Lemma logical_step_emp_intro `{!irisGS Λ Σ, !crashGS Σ} E D P :
-  P -∗
-  |~{E|D}~> P.
-Proof.
-  iIntros "HP" (R) "HR".
-  iApply (physical_step_wand with "HR"). by iIntros "$".
-Qed.
-
-Lemma logical_step_emp_use_tr_simpl `{!irisGS Λ Σ, !crashGS Σ} E D P n :
-  ⧗ n -∗
-  (|~{E|D}~> ⧗ (f n) -∗ £ (f n) -∗ P) -∗
-  |~{E|D}~> P.
-Proof.
-  iIntros "H⧗ Hstep" (R) "HR".
-  iDestruct ("Hstep" with "HR") as "HR".
-  iApply (physical_step_tr_use with "[$]").
-  iApply (physical_step_wand with "[$]").
-  iIntros "($&HP) H⧗ H£".
-  by iApply ("HP" with "[$] [$]").
-Qed.
-
-Lemma logical_step_apply `{!irisGS Λ Σ, !crashGS Σ} E D P Q :
-  (|~{E|D}~> P) -∗
-  (|={E|D}⧗=> P -∗ Q) -∗
-  |={E|D}⧗=> Q.
-Proof.
-  iIntros "Hstep HPQ".
-  iApply (physical_step_wand with "(Hstep HPQ)").
-  iIntros "[HPQ HP]". by iApply "HPQ".
-Qed.
-
 Definition wp_nval `{!irisGS Λ Σ, !crashGS Σ} E1 P :=
   ((∀ mj q g1 D κs,
        global_state_interp g1 mj D κs -∗ NC q -∗ ||={E1|⊤∖D, ∅|∅}=> ∃ D', ||={∅|∅, E1|⊤∖D'}=>
@@ -69,7 +23,7 @@ Proof.
   rewrite /wp_nval. iIntros (?????) "H HNC".
   iMod ("Hwp_nval" with "[$] [$]") as (?) "H".
   iModIntro. iExists _. iMod "H" as (?) "($&$&$&Hstep)".
-  iModIntro. iApply (logical_step_emp_wand with "[$]").
+  iModIntro. iApply (logical_step_wand with "[$]").
   iIntros "Hstep" (??) "Hg HNC".
   iMod ("Hstep" with "[$] [$]") as "($&HP&HNC)".
   rewrite ncfupd_eq /ncfupd_def. by iMod ("Hwand" with "[$] [$]") as "$".
@@ -82,7 +36,7 @@ Proof.
   iMod (fupd2_mask_subseteq ∅ ∅) as "Hclo"; [set_solver..|].
   iFrame "H". iModIntro. iMod "Hclo". iModIntro.
   iSplitR; first (iPureIntro; by left).
-  iApply logical_step_emp_intro.
+  iApply logical_step_intro.
   iIntros (??) "$ $". by iFrame.
 Qed.
 
@@ -126,7 +80,8 @@ Lemma wp_nval_wpc_nval E P :
   ▷ wp_nval E (later_tok -∗ P) -∗
   wpc_nval E P.
 Proof using later_tokG0 pri_invG0.
-  iIntros "[H⧗ H£] Hval" (E' e s Φ Φc Hnval Hsub) "Hwp".
+  iIntros "Htok Hval" (E' e s Φ Φc Hnval Hsub) "Hwp".
+  iDestruct (later_tokN_use with "[$]") as "[[?_] Hcl]".
   rewrite /wp_nval/wpc_nval.
   rewrite ?wpc_unfold /wpc_pre. iIntros (mj).
   rewrite Hnval. iSplit; last first.
@@ -141,12 +96,11 @@ Proof using later_tokG0 pri_invG0.
   iDestruct "Hstep" as (?) "(%Heq&Hg&HNC&Hstep)".
   iDestruct ("Hwp" $! mj') as "(Hwp&_)".
   iDestruct ("Hwp" with "[$] [$] [$] [//]") as "H".
-  iApply (logical_step_apply with "Hstep").
+  iMod "Hstep" as "_".
   iApply (physical_step_atomic E' (⊤∖D')). iMod "Hclo" as "_".
-  iModIntro.
-  iApply (physical_step_tr_use with "[$]").
+  iModIntro. iMod "Hcl" as "_".
   iApply (physical_step_wand with "H").
-  iIntros "(Hσ & Hg & Hwpc & Hfork & HNC) H⧗ H£ !>".
+  iIntros "(Hσ & Hg & Hwpc & Hfork & HNC) [[Htok _] _]".
   iMod (fupd_mask_subseteq E) as "Hclo"; [done..|].
   iModIntro. iIntros "Hnval".
   iMod (fupd2_mask_subseteq ∅ ∅) as "Hclo'"; [set_solver..|].
@@ -156,11 +110,7 @@ Proof using later_tokG0 pri_invG0.
   iSplitR "Hfork".
   - iApply (wpc0_mj_le'); first done.
     iApply (wpc0_strong_mono with "Hwpc"); auto. iSplit; last eauto.
-    iIntros (?) "HΦ". iModIntro. iApply "HΦ". iApply "HP".
-    assert (2 ≤ f 2).
-    { pose proof (f_exp 2); lia. }
-    iDestruct (lc_weaken with "[$]") as "$"; first done.
-    by iDestruct (tr_weaken with "[$]") as "$".
+    iIntros (?) "HΦ". iModIntro. iApply "HΦ". by iApply "HP".
   - iApply (big_sepL_mono with "[$]").
     iIntros (???) "Hwpc".
     by iApply (wpc0_mj_le').
